project/algebraic/algebraic_graph_simplification_normal.v
@@ -2,6 +2,10 @@ Require Import MyProject.project.algebraic.algebraic_graph.
 
 Require Import Recdef.
 
+
+(* This hit a wall, since rewriting to make the expression smaller again is a difficult task *)
+(* This file tries to go via some intermediate representation, but does not succeed *)
+
 Definition AG_measure {A : Type} (ag : AG A) : nat.
 Proof.
 Admitted.
